Changement de la propriet� de stabilite. Conforme au papier.

restrict2.v
@@ -3,10 +3,18 @@ Require ILLVarInt. (* Don't want import it. *)
 Import ILLVarInt.MILL. (* only this *)
 Import ILLVarInt.M. (* this *)
 Import FormulaMultiSet. (* and this *)
+Open Scope ILL_scope.
+
+(** 
+   This module contains the proof that if a sequent e ⊢ f verifies property Ap
+   (see below) then any proof h:e ⊢ f is such that Ap holds also for each node
+   of h.
+   *)
 
 
-(* This property is true when pred holds for all nodes above the root
-   of h (it has not to hold for the root). *)
+
+(** This property is true when pred holds for all nodes above the root
+   of h (it has not to hold for the root itself). *)
 Inductive Istable (pred:∀ e f (h: e ⊢ f), Prop): ∀ e f (h: e ⊢ f) , Prop := 
 | IId: ∀ Γ (f:formula) (heq:Γ == {f}), Istable pred Γ f (Id _ _ heq)
 | IImpl_R: ∀ Γ p q (h:(p :: Γ ⊢ q)), pred _ _ h → Istable pred _ _ h → Istable pred _ _ (Impl_R Γ p q h)
@@ -29,96 +37,43 @@ Inductive Istable (pred:∀ e f (h: e ⊢ f), Prop): ∀ e f (h: e ⊢ f) , Prop
 | IBang_W: ∀ Γ p q hin h, pred _ _ h → Istable pred _ _ h → (Istable pred _ _ (Bang_W Γ p q hin h)).
 
 
-
-Inductive A : formula -> Prop :=
+(** The predicate that we want to check on all
+    nodes is that formula belong to the following
+    grammar. *)
+Inductive A : formula -> Prop := (* Act *)
 | A1: A 1
 | A2:∀ φ₁ φ₂, Ac φ₁ → Ap φ₂ → A (φ₁ ⊸ φ₂)
 | A3: ∀ φ₁ φ₂, A φ₁ → A φ₂ → A (φ₁ ⊕ φ₂)
 | A4: ∀ φ₁ φ₂, A φ₁ → A φ₂ → A (φ₁ & φ₂)
 | A5: ∀ φ, A φ → A (! φ)
-with Ac: formula -> Prop:=
+with Ac: formula -> Prop:= (* CRes *)
 | Ac1: Ac 1
 | Ac2: ∀ n, Ac (Proposition n)
 | Ac3: ∀ φ₁ φ₂, Ac φ₁ → Ac φ₂ → Ac (φ₁ ⊗ φ₂)
-with Ap: formula -> Prop:=
+with Ap: formula -> Prop:= (* Context *)
 | Ap1:∀ φ, A φ → Ap φ
 | Ap2:∀ φ, R φ → Ap φ
 | Ap3: ∀ φ₁ φ₂, Ap φ₁ → Ap φ₂ → Ap (φ₁ ⊗ φ₂)
-with R: formula -> Prop:=
+with R: formula -> Prop:= (* Res *)
   R1: R 1
 | R2: ∀ n, R (Proposition n)
 | R3: ∀ φ, R φ → R (!φ)
 | R4: ∀ φ₁ φ₂, R φ₁ → R φ₂ → R (φ₁ ⊗ φ₂)
 | R5: ∀ φ₁ φ₂, R φ₁ → R φ₂ → R (φ₁ & φ₂).
 
-(*
-Lemma arrto1 : ∀ p q, arr (p ⊸ q) → arr p.
-Proof.
-  intros p q H.
-  inversion H;inversion H0;subst.
-  constructor;assumption.
-Qed.
 
-Lemma arrto2 : ∀ p q, arr (p ⊸ q) → arr q.
-Proof.
-  intros p q H.
-  inversion H;inversion H0;subst.
-  assumption.
-Qed.
+Inductive Goal : formula → Prop :=
+| G1: Goal 1
+| G2:  ∀ n, Goal (Proposition n)
+| G3: ∀ φ₁ φ₂, Goal φ₁ → Goal φ₂ → Goal (φ₁ ⊗ φ₂)
+| G4: ∀ φ₁ φ₂, Goal φ₁ → Goal φ₂ → Goal (φ₁ ⊕ φ₂)
+| G5: ∀ φ₁ φ₂, Goal φ₁ → Goal φ₂ → Goal (φ₁ & φ₂).
 
 
-Lemma arroplus1 : ∀ p q, arr (p ⊕ q) → arr p.
-Proof.
-  intros p q H.
-  inversion H;inversion H0;subst.
-  constructor;assumption.
-Qed.
-
-Lemma arroplus2 : ∀ p q, arr (p ⊕ q) → arr q.
-Proof.
-  intros p q H.
-  inversion H;inversion H0;subst.
-  constructor;assumption.
-Qed.
-
-Lemma arromult1 : ∀ p q, arr (p ⊗ q) → arr p.
-Proof.
-  intros p q H.
-  inversion H;inversion H0;subst.
-  constructor;assumption.
-Qed.
-
-Lemma arromult2 : ∀ p q, arr (p ⊗ q) → arr q.
-Proof.
-  intros p q H.
-  inversion H;inversion H0;subst.
-  constructor;assumption.
-Qed.
-
-
-
-Lemma arroesp1 : ∀ p q, arr (p & q) → arr p.
-Proof.
-  intros p q H.
-  inversion H;inversion H0;subst.
-  constructor;assumption.
-Qed.
-
-Lemma arroesp2 : ∀ p q, arr (p & q) → arr q.
-Proof.
-  intros p q H.
-  inversion H;inversion H0;subst.
-  constructor;assumption.
-Qed.
-*)
-
-Definition Apall Γ f (h:Γ⊢f):Prop := (∀g:formula, g ∈ Γ  → Ap g) /\ Ac f.
-(* Definition Aall2 Γ f (h:Γ⊢f):Prop := (∀g:formula, g ∈ Γ → A g) /\ R f. *)
-
-(* Axiom A_morph: ∀ Γ p q, Aall Γ (p ⊸ q) → A q. *)
-(* Axiom A_morph: ∀ Γ p q, Aall Γ (p ⊸ q) → A q. *)
-
-Open Scope ILL_scope.
+(** Predicate [Apall Γ f _] is true if all
+    formulas of a [Γ] are in grammar [Ap] and [f]
+    is in Goal. *)
+Definition Apall Γ f (_:Γ⊢f):Prop := (∀g:formula, g ∈ Γ  → Ap g) /\ Goal f.
 
 Lemma inEnv:∀ g p Γ,  g ∈ (p :: Γ) → g = p ∨ g ∈ Γ .
 Proof.
@@ -128,22 +83,6 @@ Proof.
   apply eq_is_eq in H1.
   auto.
 Qed.  
-
-
-(*Proof.
-  intros g p Γ H.
-
-  Set Printing All.
-  unfold add, add_multiple in H.
-  rewrite (MapsPtes.F.add_in_iff Γ p g 1%nat) in H.
-  unfold Maps'.In , Maps'.Raw.PX.In , Maps'.Raw.PX.MapsTo in H.
-  destruct  H.
-  inversion H.
-
-  unfold add, add_multiple in H0.
-  inversion H0.
-Qed.
-*)
 
 Lemma inAdd1: ∀ f Γ, f ∈ (f :: Γ) .
 Proof.
@@ -177,158 +116,6 @@ Proof.
   apply inUnion2;assumption.
 Qed.
 
-Ltac tac :=
-  match goal with
-    | H:?g ∈ ?Δ |- ?g ∈ (_ :: ?Δ ∪ _) => apply inAddUnion1;assumption
-    | H:?g ∈ ?Δ |- ?g ∈ (_ :: _ ∪ ?Δ) => apply inAddUnion2;assumption
-    | H:?g ∈ ?Δ |- ?g ∈ (?Δ ∪ _) => apply inUnion1;assumption
-    | H:?g ∈ ?Δ |- ?g ∈ (_ ∪ ?Δ) => apply inUnion2;assumption
-    | H:(R ?x) |- A ?x => constructor 2;assumption
-    | H:(R (?x ⊸ ?y)) |- _ => inversion H
-    | H:∀ g : formula, g ∈ (_ :: _ ∪ ?Δ) → A g, H':?f ∈ ?Δ |- A ?f => apply H
-    | H:∀ g : formula, g ∈ (_ :: ?Δ ∪ _) → A g, H':?f ∈ ?Δ |- A ?f => apply H
-    | H:∀ g : formula, g ∈ (_ ∪ ?Δ) → A g, H':?f ∈ ?Δ |- A ?f => apply H
-    | H:∀ g : formula, g ∈ (?Δ ∪ _) → A g, H':?f ∈ ?Δ |- A ?f => apply H
-    | H: ∀ g : formula, g ∈ (?f :: _) → A g |- A ?f => apply H
-    | H: ∀ g : formula, g ∈ (?f :: ?Γ) → A g, H': ?f' ∈ ?Γ |- A ?f' => apply H
-    | H : ∀ g : formula, g ∈ ((?p ⊸ ?q) :: ?Γ) → A g |- Ac ?p => 
-      assert (A (p ⊸ q));[ |  assert (∀ g : formula, g ∈ Γ → A g); [ intros |  clear H]]
-    | H : ∀ g : formula, g ∈ ((?p ⊸ ?q) :: ?Γ) → A g |- Ap ?q => 
-      assert (A (p ⊸ q));[ |  assert (∀ g : formula, g ∈ Γ → A g); [ intros |  clear H]]
-    | H : ∀ g : formula, g ∈ ((?p ⊗ ?q) :: ?Γ) → A g |- A ?p => 
-      assert (A (p ⊗ q));[ |  assert (∀ g : formula, g ∈ Γ → A g); [ intros |  clear H]]
-    | H : ∀ g : formula, g ∈ ((?p ⊗ ?q) :: ?Γ) → A g |- A ?q => 
-      assert (A (p ⊗ q));[ |  assert (∀ g : formula, g ∈ Γ → A g); [ intros |  clear H]]
-    | H : ∀ g : formula, g ∈ ((?p ⊕ ?q) :: ?Γ) → A g |- A ?p => 
-      assert (A (p ⊕ q));[ |  assert (∀ g : formula, g ∈ Γ → A g); [ intros |  clear H]]
-    | H : ∀ g : formula, g ∈ ((?p ⊕ ?q) :: ?Γ) → A g |- A ?q => 
-      assert (A (p ⊕ q));[ |  assert (∀ g : formula, g ∈ Γ → A g); [ intros |  clear H]]
-    | H : ∀ g : formula, g ∈ ((?p & ?q) :: ?Γ) → A g |- A ?p => 
-      assert (A (p & q));[ |  assert (∀ g : formula, g ∈ Γ → A g); [ intros |  clear H]]
-    | H : ∀ g : formula, g ∈ ((?p & ?q) :: ?Γ) → A g |- A ?q => 
-      assert (A (p & q));[ |  assert (∀ g : formula, g ∈ Γ → A g); [ intros |  clear H]]
-    | H : ∀ g : formula, g ∈ ((!?p) :: ?Γ) → A g |- A ?p => 
-      assert (A (!p));[ |  assert (∀ g : formula, g ∈ Γ → A g); [ intros |  clear H]]
-    | |- ?g ∈ (?g :: ?Γ) => apply inAdd1 (* will try stupid cases *)
-    | H:?g ∈ ?Γ |- ?g ∈ (?f :: ?Γ) => apply inAdd2;assumption
-    | H:?g ∈ (?p :: ?Γ) |- A ?g => destruct (inEnv g p Γ);auto;subst;clear H
-    | |- A (?p ⊕ ?q) => constructor
-    | |- A (?p ⊸ ?q) => constructor
-    | |- A (?p ⊗ ?q) => constructor
-    | |- A (?p & ?q) => constructor
-    | |- R ?p => constructor
-  end.
-
-(* Axiom memIn: ∀ x (y:env), Maps'.mem x y = true → Maps'.In x y. *)
-
-Lemma notA0 : ~ (A 0).
-Proof.
-  intro H.
-  inversion H.
-Qed.
-
-
-Scheme A_ind' := Induction for A Sort Prop
-with Ac_ind' := Induction for Ac Sort Prop
-with Ap_ind' := Induction for Ap Sort Prop
-with R_ind' := Induction for R Sort Prop.
-
-
-Lemma eq_A_morph: ∀ f, A f → ∀ f', ILLVarInt.MILL.eq f' f →  A f'.
-Proof.
-  intros f H.
-  induction H using A_ind' with (P0:= λ f H, ∀f', Ac f → ILLVarInt.MILL.eq f f' →  Ac f') (P1:= λ f H, ∀f', Ap f → ILLVarInt.MILL.eq f f' →  Ap f') (P2:= λ f H, ∀f', R f → ILLVarInt.MILL.eq f f' →  R f');intros.
-
-  destruct f' ;intros;simpl in *;try (subst;contradiction);  simpl in *; intuition ; constructor;auto. 
-  destruct f' ;intros;simpl in *;try (subst;contradiction);  simpl in *; intuition ; constructor;auto. 
-  destruct f' ;intros;simpl in *;try (subst;contradiction);  simpl in *; intuition ; constructor;auto. 
-  destruct f' ;intros;simpl in *;try (subst;contradiction);  simpl in *; intuition ; constructor;auto. 
-  destruct f' ;intros;simpl in *;try (subst;contradiction);  simpl in *; intuition ; constructor;auto. 
-  destruct f' ;intros;simpl in *;try (subst;contradiction);  simpl in *; intuition ; constructor;auto. 
-  destruct f' ;intros;simpl in *;try (subst;contradiction);  simpl in *; intuition ; constructor;auto. 
-  destruct f' ;intros;simpl in *;try (subst;contradiction);  simpl in *; intuition ; constructor;auto. 
-  destruct f' ;intros;simpl in *;try (subst;contradiction);  simpl in *; intuition ; constructor;auto. 
-  constructor 2. auto.
-  destruct f' ;intros;simpl in *;try (subst;contradiction);  simpl in *; intuition ; constructor 3;auto. 
-  destruct f' ;intros;simpl in *;try (subst;contradiction);  simpl in *; intuition ; constructor;auto. 
-  destruct f' ;intros;simpl in *;try (subst;contradiction);  simpl in *; intuition ; constructor;auto. 
-  destruct f' ;intros;simpl in *;try (subst;contradiction);  simpl in *; intuition ; constructor;auto. 
-  destruct f' ;intros;simpl in *;try (subst;contradiction);  simpl in *; intuition ; constructor;auto. 
-  destruct f' ;intros;simpl in *;try (subst;contradiction);  simpl in *; intuition ; constructor;auto. 
-Qed.  
-
-
-Lemma eq_Ap_morph: ∀ f, Ap f → ∀ f', ILLVarInt.MILL.eq f' f →  Ap f'.
-Proof.
-  intros f H.
-  induction H using Ap_ind' with (P:= λ f H, ∀f', A f → ILLVarInt.MILL.eq f f' →  A f') (P0:= λ f H, ∀f', Ac f → ILLVarInt.MILL.eq f f' →  Ac f') (P2:= λ f H, ∀f', R f → ILLVarInt.MILL.eq f f' →  R f');intros.
-
-  destruct f' ;intros;simpl in *;try (subst;contradiction);  simpl in *; intuition ; constructor;auto. 
-  destruct f' ;intros;simpl in *;try (subst;contradiction);  simpl in *; intuition ; constructor;auto. 
-  destruct f' ;intros;simpl in *;try (subst;contradiction);  simpl in *; intuition ; constructor;auto. 
-  destruct f' ;intros;simpl in *;try (subst;contradiction);  simpl in *; intuition ; constructor;auto. 
-  destruct f' ;intros;simpl in *;try (subst;contradiction);  simpl in *; intuition ; constructor;auto. 
-  destruct f' ;intros;simpl in *;try (subst;contradiction);  simpl in *; intuition ; constructor;auto. 
-  destruct f' ;intros;simpl in *;try (subst;contradiction);  simpl in *; intuition ; constructor;auto. 
-  destruct f' ;intros;simpl in *;try (subst;contradiction);  simpl in *; intuition ; constructor;auto. 
-  destruct f' ;intros;simpl in *;try (subst;contradiction);  simpl in *; intuition ; constructor;auto. 
-  constructor 2. auto.
-  destruct f' ;intros;simpl in *;try (subst;contradiction);  simpl in *; intuition . constructor 3;auto. 
-  destruct f' ;intros;simpl in *;try (subst;contradiction);  simpl in *; intuition ; constructor;auto. 
-  destruct f' ;intros;simpl in *;try (subst;contradiction);  simpl in *; intuition ; constructor;auto. 
-  destruct f' ;intros;simpl in *;try (subst;contradiction);  simpl in *; intuition ; constructor;auto. 
-  destruct f' ;intros;simpl in *;try (subst;contradiction);  simpl in *; intuition ; constructor;auto. 
-  destruct f' ;intros;simpl in *;try (subst;contradiction);  simpl in *; intuition ; constructor;auto. 
-Qed.  
-
-
-Lemma eq_Ac_morph: ∀ f, Ac f → ∀ f', ILLVarInt.MILL.eq f' f →  Ac f'.
-Proof.
-  intros f H.
-  induction H using Ac_ind' with (P:= λ f H, ∀f', A f → ILLVarInt.MILL.eq f f' →  A f') (P1:= λ f H, ∀f', Ap f → ILLVarInt.MILL.eq f f' →  Ap f') (P2:= λ f H, ∀f', R f → ILLVarInt.MILL.eq f f' →  R f');intros.
-
-  destruct f' ;intros;simpl in *;try (subst;contradiction);  simpl in *; intuition ; constructor;auto. 
-  destruct f' ;intros;simpl in *;try (subst;contradiction);  simpl in *; intuition ; constructor;auto. 
-  destruct f' ;intros;simpl in *;try (subst;contradiction);  simpl in *; intuition ; constructor;auto. 
-  destruct f' ;intros;simpl in *;try (subst;contradiction);  simpl in *; intuition ; constructor;auto. 
-  destruct f' ;intros;simpl in *;try (subst;contradiction);  simpl in *; intuition ; constructor;auto. 
-  destruct f' ;intros;simpl in *;try (subst;contradiction);  simpl in *; intuition ; constructor;auto. 
-  destruct f' ;intros;simpl in *;try (subst;contradiction);  simpl in *; intuition ; constructor;auto. 
-  destruct f' ;intros;simpl in *;try (subst;contradiction);  simpl in *; intuition ; constructor;auto. 
-  destruct f' ;intros;simpl in *;try (subst;contradiction);  simpl in *; intuition ; constructor;auto. 
-  constructor 2. auto.
-  destruct f' ;intros;simpl in *;try (subst;contradiction);  simpl in *; intuition . constructor 3;auto. 
-  destruct f' ;intros;simpl in *;try (subst;contradiction);  simpl in *; intuition ; constructor;auto. 
-  destruct f' ;intros;simpl in *;try (subst;contradiction);  simpl in *; intuition ; constructor;auto. 
-  destruct f' ;intros;simpl in *;try (subst;contradiction);  simpl in *; intuition ; constructor;auto. 
-  destruct f' ;intros;simpl in *;try (subst;contradiction);  simpl in *; intuition ; constructor;auto. 
-  destruct f' ;intros;simpl in *;try (subst;contradiction);  simpl in *; intuition ; constructor;auto. 
-Qed.  
-
-Lemma eq_R_morph: ∀ f, R f → ∀ f', ILLVarInt.MILL.eq f' f →  R f'.
-Proof.
-  intros f H.
-  induction H using R_ind' with (P:= λ f H, ∀f', A f → ILLVarInt.MILL.eq f f' →  A f') (P1:= λ f H, ∀f', Ap f → ILLVarInt.MILL.eq f f' →  Ap f') (P0:= λ f H, ∀f', Ac f → ILLVarInt.MILL.eq f f' →  Ac f');intros.
-
-  destruct f' ;intros;simpl in *;try (subst;contradiction);  simpl in *; intuition ; constructor;auto. 
-  destruct f' ;intros;simpl in *;try (subst;contradiction);  simpl in *; intuition ; constructor;auto. 
-  destruct f' ;intros;simpl in *;try (subst;contradiction);  simpl in *; intuition ; constructor;auto. 
-  destruct f' ;intros;simpl in *;try (subst;contradiction);  simpl in *; intuition ; constructor;auto. 
-  destruct f' ;intros;simpl in *;try (subst;contradiction);  simpl in *; intuition ; constructor;auto. 
-  destruct f' ;intros;simpl in *;try (subst;contradiction);  simpl in *; intuition ; constructor;auto. 
-  destruct f' ;intros;simpl in *;try (subst;contradiction);  simpl in *; intuition ; constructor;auto. 
-  destruct f' ;intros;simpl in *;try (subst;contradiction);  simpl in *; intuition ; constructor;auto. 
-  destruct f' ;intros;simpl in *;try (subst;contradiction);  simpl in *; intuition ; constructor;auto. 
-  constructor 2. auto.
-  destruct f' ;intros;simpl in *;try (subst;contradiction);  simpl in *; intuition . constructor 3;auto. 
-  destruct f' ;intros;simpl in *;try (subst;contradiction);  simpl in *; intuition ; constructor;auto. 
-  destruct f' ;intros;simpl in *;try (subst;contradiction);  simpl in *; intuition ; constructor;auto. 
-  destruct f' ;intros;simpl in *;try (subst;contradiction);  simpl in *; intuition ; constructor;auto. 
-  destruct f' ;intros;simpl in *;try (subst;contradiction);  simpl in *; intuition ; constructor;auto. 
-  destruct f' ;intros;simpl in *;try (subst;contradiction);  simpl in *; intuition ; constructor;auto. 
-Qed.  
-
-
 Lemma mem_remove: ∀ Γ f Δ g,  Γ \ f == Δ → g ∈ Δ → g ∈ Γ.
 Proof.
   intros Γ f Δ g H H0.
@@ -347,28 +134,44 @@ Proof.
   constructor 3;assumption.
 Qed.
 
+Lemma Ap_Goal: ∀x, Ac x → Goal x.
+Proof.
+  intros x H.
+  induction H.
+  constructor.
+  constructor.
+  constructor;assumption.
+Qed.
+
+
+
 Ltac zap := 
   match goal with
     | |- ?x == ?x => apply eq_refl
     | H: ILLVarInt.MILL.eq ?g ?q |- _ => apply eq_is_eq in H;subst
     | H:?g ∈ (?q :: ?D') |- _ => destruct (mem_destruct _ _ _ H);clear H
     | H: ?p ∈ ?Γ ,  H':∀ g : formula, g ∈ ?Γ → Ap g |- _ => assert (Ap (p)) by auto;clear H
+    | H: Ac ?p |- Goal ?p => apply Ap_Goal;assumption
     | H:Ap (?p ⊸ ?q) |- _ => inversion H;clear H
     | H:A (?p ⊸ ?q) |- _ => inversion H;clear H
     | H:R (?p ⊸ ?q) |- _ => inversion H;clear H
     | H:Ac (?p ⊸ ?q) |- _ => inversion H;clear H
+    | H:Goal (?p ⊸ ?q) |- _ => inversion H;clear H
     | H:Ap (?p ⊕ ?q) |- _ => inversion H;clear H
     | H:A (?p ⊕ ?q) |- _ => inversion H;clear H
     | H:R (?p ⊕ ?q) |- _ => inversion H;clear H
     | H:Ac (?p ⊕ ?q) |- _ => inversion H;clear H
+    | H:Goal (?p ⊕ ?q) |- _ => inversion H;clear H
     | H:Ap (?p ⊗ ?q) |- _ => inversion H;clear H
     | H:A (?p ⊗ ?q) |- _ => inversion H;clear H
     | H:R (?p ⊗ ?q) |- _ => inversion H;clear H
     | H:Ac (?p ⊗ ?q) |- _ => inversion H;clear H
+    | H:Goal (?p ⊗ ?q) |- _ => inversion H;clear H
     | H:Ap (?p & ?q) |- _ => inversion H;clear H
     | H:A (?p & ?q) |- _ => inversion H;clear H
     | H:R (?p & ?q) |- _ => inversion H;clear H
     | H:Ac (?p & ?q) |- _ => inversion H;clear H
+    | H:Goal (?p & ?q) |- _ => inversion H;clear H
     | H: ?g ∈ ?Δ |- ?g ∈ (?Δ ∪ ?Δ') => apply mem_union_l;assumption
     | H: ?g ∈ ?Δ |- ?g ∈ (?Δ' ∪ ?Δ) => apply mem_union_r;assumption
     | H: ILLVarInt.MILL.eq ?g ?q |- _ => apply eq_is_eq in H;subst
@@ -414,6 +217,16 @@ Proof.
   apply essai;split;intros;repeat (zap;subst);apply H0;repeat zap.
   Guarded.
 
+  apply essai;split;intros;repeat (zap;subst);apply H0;repeat zap.
+  Guarded.
+
+  apply essai;split;intros;repeat (zap;subst);apply H0;repeat zap.
+  Guarded.
+
+  apply essai;split;intros;repeat (zap;subst);apply H0;repeat zap.
+  Guarded.
+  apply essai;split;intros;repeat (zap;subst);apply H0;repeat zap.
+  Guarded.
   apply essai;split;intros;repeat (zap;subst);apply H0;repeat zap.
   Guarded.
 
